#import "@preview/rubber-article:0.3.1": maketitle, article

#show: article.with(lang: "he", heading-numbering: none)

#show math.equation.where(block: true): set block(breakable: true)
#show math.equation.where(block: false): box
#set text(font: "David CLM")

#let ds = $. space$
#let mtext = text.with(font: "David CLM")
#let Span = math.op[Span]
#let amat = math.mat.with(augment: -1)
#let tab = $space space space space$

#maketitle(
  title: "אלגברה לינארית 1א - תרגיל בית 2",
  authors: ("דניאל פ.ח.",),
  date: datetime(day: 7, month: 4, year: 2025).display("[day].[month].[year]"),
)

= שאלה 1

== סעיף א

אם
$a = 0 or b = 0$,
נניח בה"כ
$a = 0$
ואז:

$
  b^2 = 0 \
  b dot b = 0 \
  b = 0 or b = 0 \
  b = 0 \
  b = a \
$

אחרת:

$
  a^2 = b^2 \
  a^2 - b^2 = 0 \
  a^2 + a dot b - a dot b - b^2 = 0 \
  a dot (a + b) - (a + b) dot b = 0 \
  (a + b)(a - b) = 0 \
  a + b = 0 or a - b = 0 \
  a = -b or a = b \
$

== סעיף ב

$
  0 dot b = 0 dot (-b) \
  (a + (-a)) dot b = (a + (-a)) dot (-b) \
  a dot b + (-a) dot b = a dot (-b) + (-a) dot (-b) \
  a dot b + (-a) dot b + (-(a dot (-b))) = (-a) dot (-b) \
  a dot b + (-a) dot b + (-a) dot (-b) = (-a) dot (-b) \
  a dot b + (-a) dot (b +(-b)) = (-a) dot (-b) \
  a dot b + (-a) dot 0 = (-a) dot (-b) \
  a dot b = (-a) dot (-b) \
$

== סעיף ג

הוכחת עזר:

$
  (a dot b) dot (a^(-1) dot b^(-1))
  = (a dot a^(-1)) dot (b dot b^(-1))
  = 1 dot 1
  = 1 \
  arrow.b.double \
  a^(-1) dot b^(-1) = (a dot b)^(-1)
$

הוכחה:

$
  a dot b^(-1) + c dot d^(-1)
  &= (a dot b^(-1)) dot 1 + (c dot d^(-1)) dot 1 \
  &= (a dot b^(-1)) dot (d dot d^(-1)) + (c dot d^(-1)) dot (b dot b^(-1)) \
  &= (a dot d) dot (b^(-1) dot d^(-1)) + (c dot b) dot (d^(-1) dot b^(-1)) \
  mtext("מהוכחת העזר") arrow.r space
  &= (a dot d) dot (b dot d)^(-1) + (c dot b) dot (d dot b)^(-1) \
  &= (a dot d + c dot b) dot (d dot b)^(-1) \
$

= שאלה 2

== סעיף א

לכל
$x in {1, ..., p-1}$
מתקיים
$x^(-1) in {1, ..., p-1}$,
בנוסף
$(x^(-1))^(-1) = x$,
לכן:

$
  product_(i=1)^(p-1) i = product_(i=1)^(p-1) i^(-1)
$

זאת ועוד, לא קיימים
$x != y in {1, ..., p-1}$
שונים כך ש-$x^(-1) = y^(-1)$,
לכן:

$
  I_2 = { i^(-1) | i in I_1 }
$

כאשר:

$
  I_1 = { i < i^(-1) | i in {1, ..., p-1} } \
  I_2 = { i > i^(-1) | i in {1, ..., p-1} } \
$

לבסוף, נשים לב ש-

$
  I_3 = {1, p-1}
$

כאשר:

$
  I_3 = { i = i^(-1) | i in {1, ..., p-1} }
$

וסה"כ:

$
  product_(i=1)^(p-1) i
  &= product_(i in I_1) i dot product_(i in I_2) i dot product_(i in I_3) i \
  &= product_(i in I_1) i dot product_(i in I_1) i^(-1) dot product_(i in {1,p-1}) i \
  &= (product_(i in I_1) i dot i^(-1)) dot 1 dot (p-1) \
  &= (product_(i in I_1) 1) dot (-1) \
  &= 1 dot (-1) \
  &= -1 \
$

== סעיף ב

מסעיף א:

$
  (p-1)! eq.triple#[]_p -1 \
  <=> exists k in NN. ((p-1)! - (-1)) = p dot k \
  <=> exists k in NN. ((p-1)! + 1) = p dot k \
  <=> exists k in NN. (1 + (p-1)!) = p dot k \
$

= שאלה 4

== סעיף א

$
  amat(
    3, 2, -1, 1, 7;
    2, 1, -3, -1, 11;
  ) \
  R_1 => R_1 + R_2 \
  amat(
    5, 3, -4, 0, 18;
    2, 1, -3, -1, 11;
  ) \
  R_2 => R_2 - 3 / 4 R_1 \
  amat(
    5, 3, -4, 0, 18;
    -7/4, -5/4, 0, -1, -5/2;
  ) \
  R_1 => R_1 / (-4) \
  R_2 => R_2 / (-1) \
  amat(
    -5/4, -3/4, 1, 0, -9/2;
    7/4, 5/4, 0, 1, 5/2;
  ) \
  cases(
    -5/4 x_1 + -3/4 x_2 + x_3 = -9/2,
    7/4 x_1 + 5/4 x_2 + x_4 = 5/2,
  ) \
  cases(
    x_3 = -9/2 + 5/4 x_1 + 3/4 x_2,
    x_4 = 5/2 - 7/4 x_1 - 5/4 x_2,
  ) \
$

$x_1, x_2$
משתנים חופשיים.

== סעיף ב

$
  amat(
    3, 2, 2, 2, 2;
    2, 3, 2, 5, 3;
    9, 1, 4, -5, 1;
    2, 2, 3, 4, 5;
    7, 1, 6, -4, 7;
  ) \
  R_2 => R_1 / 2 \
  amat(
    3, 2, 2, 2, 2;
    1, 3/2, 1, 5/2, 3/2;
    9, 1, 4, -5, 1;
    2, 2, 3, 4, 5;
    7, 1, 6, -4, 7;
  ) \
  R_1 => R_1 - 3R_2 \
  R_3 => R_3 - 9R_2 \
  R_4 => R_4 - 2R_2 \
  R_5 => R_5 - 7R_2 \
  amat(
    0, -5/2, 1, -11/2, -5/2;
    1, 3/2, 1, 5/2, 3/2;
    0, -25/2, -5, -55/2, -25/2;
    0, -1, 1, -1, 2;
    0, -19/2, -1, -43/2, -7/2;
  ) \
  R_4 => -R_4 \
  amat(
    0, -5/2, 1, -11/2, -5/2;
    1, 3/2, 1, 5/2, 3/2;
    0, -25/2, -5, -55/2, -25/2;
    0, 1, -1, 1, -2;
    0, -19/2, -1, -43/2, -7/2;
  ) \
  R_1 => R_1 + 5 / 2R_4 \
  R_2 => R_2 - 3 / 2R_4 \
  R_3 => R_3 + 25 / 2R_4 \
  R_5 => R_5 + 19 / 2R_4 \
  amat(
    0, 0, -3/2, -6/2, -15/2;
    1, 0, 5/2, 1, 9/2;
    0, 0, -35/2, 5/2, -105/2;
    0, 1, -1, 1, -2;
    0, 0, -21/2, -24/2, -45/2;
  ) \
  R_1 => R_1 / (-3 / 2) \
  amat(
    0, 0, 1, 2, 3;
    1, 0, 5/2, 1, 9/2;
    0, 0, -35/2, 5/2, -105/2;
    0, 1, -1, 1, -2;
    0, 0, -21/2, -24/2, -45/2;
  ) \
  R_2 => R_2 - 5 / 2R_1 \
  R_3 => R_3 + 35 / 2R_1 \
  R_4 => R_4 + R_1 \
  R_5 => R_5 + 21 / 2R_1 \
  amat(
    0, 0, 1, 2, 3;
    1, 0, 0, -8/2, -6/2;
    0, 0, 0, 65/2, -10/2;
    0, 1, 0, 3, 1;
    0, 0, 0, -1, 9;
  ) \
  R_5 => R_5 / (-1) \
  amat(
    0, 0, 1, 2, 3;
    1, 0, 0, -8/2, -6/2;
    0, 0, 0, 65/2, -10/2;
    0, 1, 0, 3, 1;
    0, 0, 0, 1, -9;
  ) \
  R_1 => R_1 - 2R_5 \
  R_2 => R_2 + 8 / 2R_5 \
  R_3 => R_3 - 65 / 2R_5 \
  R_4 => R_4 - 3R_1 \
  amat(
    0, 0, 1, 0, 21;
    1, 0, 0, 0, -39;
    0, 0, 0, 0, -575/2;
    0, 1, 0, 0, 26;
    0, 0, 0, 1, -9;
  ) \
  R_1 <=> R_2 \
  amat(
    1, 0, 0, 0, -39;
    0, 0, 1, 0, 21;
    0, 0, 0, 0, -575/2;
    0, 1, 0, 0, 26;
    0, 0, 0, 1, -9;
  ) \
  R_3 <=> R_4 \
  amat(
    1, 0, 0, 0, -39;
    0, 0, 1, 0, 21;
    0, 1, 0, 0, 26;
    0, 0, 0, 0, -575/2;
    0, 0, 0, 1, -9;
  ) \
  R_2 <=> R_3 \
  amat(
    1, 0, 0, 0, -39;
    0, 1, 0, 0, 26;
    0, 0, 1, 0, 21;
    0, 0, 0, 0, -575/2;
    0, 0, 0, 1, -9;
  ) \
  R_4 <=> R_5 \
  amat(
    1, 0, 0, 0, -39;
    0, 1, 0, 0, 26;
    0, 0, 1, 0, 21;
    0, 0, 0, 1, -9;
    0, 0, 0, 0, -575/2;
  ) \
  cases(
    x_1 + = -39,
    x_2 = 26,
    x_3 = 21,
    x_4 = -9,
    0 = -575/2,
  ) \
$

אין פתרון.

== סעיף ג

$
  amat(
    2, 3, 4, 3;
    3, -2, 5, 10;
    7, 9, 3, 1;
  ) \
  R_1 => R_1 / 2 \
  amat(
    1, 3/2, 2, 3/2;
    3, -2, 5, 10;
    7, 9, 3, 1;
  ) \
  R_2 => R_2 - 3R_1 \
  R_3 => R_3 - 7R_1 \
  amat(
    1, 3/2, 2, 3/2;
    0, -13/2, -1, 11/2;
    0, -3/2, -11, -19/2;
  ) \
  R_3 => R_3 / (-3 / 2) \
  amat(
    1, 3/2, 2, 3/2;
    0, -13/2, -1, 11/2;
    0, 1, 22/3, 19/3;
  ) \
  R_1 => R_1 - 3 / 2 \
  R_2 => R_2 + 13 / 2 \
  amat(
    1, 0, -9, -16/2;
    0, 0, 140/3, 71/6;
    0, 1, 22/3, 19/3;
  ) \
  R_2 => R_2 / (140 / 2) \
  amat(
    1, 0, -9, -16/2;
    0, 0, 1, 71/420;
    0, 1, 22/3, 19/3;
  ) \
  R_1 => R_1 + 9R_2 \
  R_3 => R_3 - 22 / 3R_1 \
  amat(
    1, 0, 0, -907/140;
    0, 0, 1, 71/420;
    0, 1, 0, 3209/630;
  ) \
  R_2 <=> R_3 \
  amat(
    1, 0, 0, -907/140;
    0, 1, 0, 3209/630;
    0, 0, 1, 71/420;
  ) \
  cases(
    x_1 = -907/140,
    x_2 = 3209/630,
    x_3 = 71/420,
  ) \
$

אין משתנים חופשיים.

= שאלה 5

$
  amat(
    3, 2, 4, 1, 2;
    2, 1, 2, 4, 1;
  ) \
  R_1 => R_1 / 3 \
  amat(
    1, 4, 3, 2, 4;
    2, 1, 2, 4, 1;
  ) \
  R_2 => R_2 - 2R_1 \
  amat(
    1, 4, 3, 2, 4;
    0, 3, 1, 0, 3;
  ) \
  R_2 => R_2 / 3 \
  amat(
    1, 4, 3, 2, 4;
    0, 1, 2, 0, 1;
  ) \
  R_1 => R_1 - 4R_2 \
  amat(
    1, 0, 0, 2, 0;
    0, 1, 2, 0, 1;
  ) \
  cases(
    x_1 + x_4 = 0,
    x_2 + 2x_3 = 1,
  ) \
  cases(
    x_1 = -x_4,
    x_2 = 1 - 2x_3,
  ) \
$

$x_4, x_3$
משתנים חופשיים.

== סעיף ב

$
  amat(
    3, 2, 4, 1, 2;
    2, 1, 2, 4, 1;
  ) \
  R_1 => R_1 / 3 \
  amat(
    1, 3, 6, 5, 3;
    2, 1, 2, 4, 1;
  ) \
  R_2 => R_2 - 2R_1 \
  amat(
    1, 3, 6, 5, 3;
    0, 2, 4, 1, 2;
  ) \
  R_2 => R_2 / 2 \
  amat(
    1, 3, 6, 5, 3;
    0, 1, 2, 4, 1;
  ) \
  R_1 => R_1 - 3R_2 \
  amat(
    1, 0, 0, 0, 0;
    0, 1, 2, 4, 1;
  ) \
  cases(
    x_1 = 0,
    x_2 + x_3 + x_4 = 1,
  ) \
  cases(
    x_1 = 0,
    x_2 = 1 - x_3 - x_4,
  ) \
$

$x_3, x_4$
משתנים חופשיים.

== סעיף ג

$
  amat(
    1, 2, 3, 4, 0;
    1, i, -1, -i, 1;
  ) \
  R_2 => R_2 - R_1 \
  amat(
    1, 2, 3, 4, 0;
    0, i-2, -4, -i-4, 1;
  ) \
  R_2 => R_2 / (i-2) \
  amat(
    1, 2, 3, 4, 0;
    0, 1, 8/5-4/5i, 7/5+6/5i, -2/5+1/5i;
  ) \
  R_1 => R_1 - 2R_2 \
  amat(
    1, 0, -1/5+8/5i, 6/5-6/5i, 4/5-2/5i;
    0, 1, 8/5-4/5i, 7/5+6/5i, -2/5+1/5i;
  ) \
  amat(
    1, 0, (-1+8i)/5, (6-6i)/5, (4-2i)/5;
    0, 1, (8-4i)/5, (7+6i)/5, (-2+i)/5;
  ) \
  cases(
    x_1 + (-1+8i)/5x_3 + (6-6i)/5x_4 = (4-2i)/5,
    x_2 + (8-4i)/5x_3 + (7+6i)/5x_4 = (-2+i)/5,
  ) \
  cases(
    x_1 = (4-2i)/5 - (-1+8i)/5x_3 - (6-6i)/5x_4,
    x_2 = (-2+i)/5 - (8-4i)/5x_3 - (7+6i)/5x_4,
  ) \
$

$x_3,x_4$
משתנים חופשיים.

== סעיף ד

$
  amat(
    1, 1, 0, 1, 0, 1;
    1, 0, 1, 1, 0, 0;
    0, 1, 0, 1, 1, 0;
  ) \
  R_2 => R_2 - R_1 \
  amat(
    1, 1, 0, 1, 0, 1;
    0, 1, 1, 0, 0, 1;
    0, 1, 0, 1, 1, 0;
  ) \
  R_1 => R_1 - R_2 \
  R_3 => R_3 - R_2 \
  amat(
    1, 0, 1, 1, 0, 0;
    0, 1, 1, 0, 0, 1;
    0, 0, 1, 1, 1, 1;
  ) \
  R_1 => R_1 - R_3 \
  R_2 => R_2 - R_3 \
  amat(
    1, 0, 0, 0, 1, 1;
    0, 1, 0, 1, 1, 0;
    0, 0, 1, 1, 1, 1;
  ) \
  cases(
    x_1 + x_4 = 1,
    x_2 + x_4 + x_5 = 0,
    x_3 + x_4 + x_5 = 1,
  ) \
  cases(
    x_1 = 1 - x_4,
    x_2 = -x_4 - x_5,
    x_3 = 1 - x_4 - x_5,
  ) \
  cases(
    x_1 = 1 + x_4,
    x_2 = 0 + x_4 + x_5,
    x_3 = 1 + x_4 + x_5,
  ) \
$

$x_4, x_5$
משתנים חופשיים.


= שאלה 6

== סעיף א

$
  { mat(
      1, 0;
      0, 1;
    )} union { mat(
      1, a;
      0, 0;
    ) | a in FF} union { mat(
      0, 1;
      0, 0;
    ) }
$

== סעיף ב

$
  &{ mat(
      1, 0, 0;
      0, 1, 0;
      0, 0, 1;
    ) } union { mat(
      1, 0, a;
      0, 1, b;
      0, 0, 0;
    ) | a,b in FF } union { mat(
        1, a, 0;
        0, 0, 1;
        0, 0, 0;
      ) | a in FF } \
  &tab union { mat(
        1, a, b;
        0, 0, 0;
        0, 0, 0;
      ) | a, b in FF } union { mat(
        0, 1, 0;
        0, 0, 1;
        0, 0, 0;
      ) } union { mat(
        0, 1, a;
        0, 0, 0;
        0, 0, 0;
      ) | a in FF } union { mat(
        0, 0, 1;
        0, 0, 0;
        0, 0, 0;
      ) }
$
